Adding lower layers with lock logic to async set copy

examples/async_set_copy.bpl
@@ -4,13 +4,78 @@
  * Copyright (c) 2019, Oracle and/or its affiliates. All rights reserved.
  */
 
+// =============================================================================
 // Linear thread identifiers
+// =============================================================================
 type Tid;
 function {:builtin "MapConst"} MapConstTidBool(bool) : [Tid]bool;
 function {:inline}{:linear "tid"} TidCollector(tid:Tid) : [Tid]bool
 {
   MapConstTidBool(false)[tid := true]
 }
+type TidSet = [Tid]bool;
+function EmptyTidSet() : TidSet
+{ (lambda t : Tid :: false) }
+
+
+// =============================================================================
+// A lock is a record consisting of a flag indicating whether the lock
+// is held in exclusive or shared mode and a set of thread identifiers
+// who hold the lock. The associated atomic steps AcquireLock{Shared,Exclusive}
+// and ReleaseLock{Shared,Exclusive} maintain the invariant that a lock
+// held in exclusive mode has exactly one holder, i.e. tids contains
+// exactly one element.
+// =============================================================================
+type {:datatype} Lock;
+function {:constructor} Lock(exclusive : bool, tids: TidSet) : Lock;
+
+var {:layer 0, 5} lock : Lock;
+
+procedure {:yields} {:layer 0} {:refines "A_AcquireLockShared"} AcquireLockShared({:linear "tid"} tid: Tid);
+procedure {:right} {:layer 1, 5} A_AcquireLockShared({:linear "tid"} tid: Tid)
+modifies lock;
+{
+  assume !exclusive#Lock(lock) && !tids#Lock(lock)[tid];
+  lock := Lock(false, tids#Lock(lock)[tid:=true]);
+}
+
+procedure {:yields} {:layer 0} {:refines "A_AcquireLockExclusive"} AcquireLockExclusive({:linear "tid"} tid: Tid);
+procedure {:right} {:layer 1, 5} A_AcquireLockExclusive({:linear "tid"} tid: Tid)
+modifies lock;
+{
+  assume !exclusive#Lock(lock) && tids#Lock(lock) == EmptyTidSet();
+  lock := Lock(true, tids#Lock(lock)[tid:=true]);
+}
+
+function HoldsLock(tid: Tid, lock: Lock) : bool
+{
+  tids#Lock(lock)[tid]
+}
+
+procedure {:yields} {:layer 0} {:refines "A_ReleaseLockShared"} ReleaseLockShared({:linear "tid"} tid: Tid);
+procedure {:left} {:layer 1, 5} A_ReleaseLockShared({:linear "tid"} tid: Tid)
+modifies lock;
+{
+  assert !exclusive#Lock(lock) && HoldsLock(tid, lock);
+  lock := Lock(false, tids#Lock(lock)[tid:=true]);
+}
+
+function HoldsLockExclusive(tid: Tid, lock: Lock) : bool
+{
+  exclusive#Lock(lock) && tids#Lock(lock) == EmptyTidSet()[tid:=true]
+}
+
+procedure {:yields} {:layer 0} {:refines "A_ReleaseLockExclusive"} ReleaseLockExclusive({:linear "tid"} tid: Tid);
+procedure {:left} {:layer 1, 5} A_ReleaseLockExclusive({:linear "tid"} tid: Tid)
+modifies lock;
+{
+  assert HoldsLockExclusive(tid, lock);
+  lock := Lock(false, EmptyTidSet());
+}
+
+// =============================================================================
+// The algorithm
+// =============================================================================
 
 type SetInt = [int]bool;
 
@@ -22,7 +87,11 @@ var {:layer 0, 10} requested_copy_bound : int;
 var {:layer 0, 10} copy_thread : Tid;
 
 var {:layer 0, 10} is_running : [Tid]bool; 
-var {:layer 0, 10} N: int;
+var {:layer 0, 10} N : int;
+
+// =============================================================================
+// Main
+// =============================================================================
 
 // Models the large atomic step in the body of main. In the actual implementation,
 // this atomic step asynchronously calls Write and potentially Copy. I don't know
@@ -34,7 +103,6 @@ procedure {:atomic} {:layer 1,10} A_MainBody()
 modifies requested_copy_bound, is_running, copy_thread, N;
 {
   assert requested_copy_bound <= N;
-  assert copy_bound <= requested_copy_bound;
   // async call Write(N+1);
   if (*) {
     requested_copy_bound := N;
@@ -76,6 +144,10 @@ requires {:layer 0, 10} copy_bound == 0;
   yield;
 } 
 
+// =============================================================================
+// Write
+// =============================================================================
+
 // First atomic step in Write
 //
 // The actual implementation only waits for !is_running[copy_thread], but it is sound
@@ -88,9 +160,52 @@ procedure {:right} {:layer 1, 10} A_WaitNotRunning(n: int)
   assume !is_running[copy_thread] || n <= requested_copy_bound;
 }
 
+// Returns copy_bound
+procedure {:yields} {:layer 0} {:refines "A_Get_Copy_Bound"} Get_Copy_Bound({:linear "tid"} tid: Tid) returns (c : int);
+procedure {:both} {:layer 1, 5} A_Get_Copy_Bound({:linear "tid"} tid: Tid) returns (c : int)
+{
+  assert HoldsLock(tid, lock);
+  c := copy_bound;
+}
+
+// Add an element to the set copy
+// Requires a shared lock so that this is a both mover
+procedure {:yields} {:layer 0} {:refines "A_AddToCopy"} AddToCopy({:linear "tid"} tid: Tid, n: int);
+procedure {:both} {:layer 1, 5} A_AddToCopy({:linear "tid"} tid: Tid, n: int)
+modifies copy;
+{
+  assert HoldsLock(tid, lock);
+  copy := copy[n:=true];
+}
+
+// Add an element to the set latest
+// Requires a shared lock so that this is a both mover
+procedure {:yields} {:layer 0} {:refines "A_AddToLatest"} AddToLatest({:linear "tid"} tid: Tid, n: int);
+procedure {:both} {:layer 1, 5} A_AddToLatest({:linear "tid"} tid: Tid, n: int)
+modifies latest;
+{
+  assert HoldsLock(tid, lock);
+  latest := latest[n:=true];
+}
+
+// Implementation of writing to latest and potentially to copy.
+// Shared lock allows the two writes to be treated as one atomic step.
+procedure {:yields} {:layer 5} {:refines "A_DoWrite"} DoWrite({:linear "tid"} tid: Tid, n: int)
+{
+  var local_copy_bound : int;
+  yield;
+  call AcquireLockShared(tid);
+  call local_copy_bound := Get_Copy_Bound(tid);
+  if (n <= local_copy_bound) {
+    call AddToCopy(tid, n);
+  }
+  call AddToLatest(tid, n);
+  call ReleaseLockShared(tid);
+  yield;
+}
+
 // Second atomic step in Write, after using and eliminating the lock.
-procedure {:yields} {:layer 5} {:refines "A_DoWrite"} DoWrite(n: int);
-procedure {:atomic} {:layer 6, 10} A_DoWrite(n: int)
+procedure {:atomic} {:layer 6, 10} A_DoWrite({:linear "tid"} tid: Tid, n: int)
 modifies copy, latest;
 {
   assert is_running[copy_thread] ==> n <= requested_copy_bound;
@@ -104,20 +219,20 @@ modifies copy, latest;
 //
 // Write is asynchronously called with an argument (N+1), but the same atomic step
 // also increments N after calling Write, so the precondition n <= N does hold.
-procedure {:yields} {:layer 6} {:refines "A_Write"} Write(n: int)
+procedure {:yields} {:layer 6} {:refines "A_Write"} Write({:linear "tid"} tid: Tid,  n: int)
 requires {:layer 6} n <= N;
 {
   yield;
   assert {:layer 6} n <= N;
 
   call WaitNotRunning(n);
-  call DoWrite(n);
+  call DoWrite(tid, n);
   yield;
 }
 
 // Atomic summary of Write, basically just gets rid of the wait for
 // !is_running[copy_thread];
-procedure {:atomic} {:layer 7, 10} A_Write(n: int)
+procedure {:atomic} {:layer 7, 10} A_Write({:linear "tid"} tid: Tid, n: int)
 modifies copy, latest;
 {
   assume !is_running[copy_thread] || n <= requested_copy_bound;
@@ -127,10 +242,14 @@ modifies copy, latest;
   latest := latest[n:=true];
 }
 
+// =============================================================================
+// Copy
+// =============================================================================
+
 // Models evaluating the loop condition in Copy to true.
 procedure {:yields} {:layer 0} {:refines "A_Copy_Continue"}
   Copy_Continue(creating_copy_bound: int) returns (next_copy_bound: int);   
-procedure {:right} {:layer 1, 6} A_Copy_Continue(creating_copy_bound: int)
+procedure {:right} {:layer 1, 5} A_Copy_Continue(creating_copy_bound: int)
   returns (next_copy_bound: int)
 {
   assert creating_copy_bound <= requested_copy_bound;
@@ -143,11 +262,44 @@ procedure {:right} {:layer 1, 6} A_Copy_Continue(creating_copy_bound: int)
 // sets is_running to false. This is actually necessary for correctness.
 procedure {:yields} {:layer 0} {:refines "A_Copy_Stop"}
   Copy_Stop(tid: Tid, creating_copy_bound: int);
-procedure {:atomic} {:layer 1, 6} A_Copy_Stop(tid: Tid, creating_copy_bound: int)
+procedure {:atomic} {:layer 1, 5} A_Copy_Stop(tid: Tid, creating_copy_bound: int)
 modifies is_running;
 {
   assume creating_copy_bound == requested_copy_bound;
   is_running := is_running[tid:=false];
+}
+
+// Initialize copy by setting it to latest
+// Requires exclusive lock to be a both mover
+procedure {:yields} {:layer 0} {:refines "A_CreateCopy"} CreateCopy({:linear "tid"} tid: Tid);
+procedure {:both} {:layer 1, 4} A_CreateCopy({:linear "tid"} tid: Tid)
+modifies copy;
+{
+  assert HoldsLockExclusive(tid, lock);
+  copy := latest;
+}
+
+// Set copy_bound to n
+// Requires exclusive lock to be a both mover
+procedure {:yields} {:layer 0} {:refines "A_Set_Copy_Bound"} Set_Copy_Bound({:linear "tid"} tid: Tid, n: int);
+procedure {:both} {:layer 1, 4} A_Set_Copy_Bound({:linear "tid"} tid: Tid, n: int)
+modifies copy_bound;
+{
+  assert HoldsLockExclusive(tid, lock);
+  copy_bound := n;
+}
+
+// Yielding procedure that does the actual copy and copy_bound work in Copy.
+procedure {:yields} {:layer 4} {:refines "A_DoCopy"}
+  DoCopy({:linear "tid"} tid: Tid, creating_copy_bound: int)
+requires {:layer 4} HoldsLockExclusive(tid, lock);
+ensures {:layer 4} HoldsLockExclusive(tid, lock);
+{
+  yield;
+  call CreateCopy(tid);
+  call Set_Copy_Bound(tid, creating_copy_bound);
+  yield;
+  assert {:layer 4} HoldsLockExclusive(tid, lock);
 }
 
 // Generalization of the part of the body of Copy that sets copy and copy_bound.
@@ -167,15 +319,14 @@ modifies is_running;
 // the algorithm, so that will have to be addressed at a lower layer. Decoupling
 // crash safety from other correctness properties seems to be a benefit of the
 // CIVL approach.
-procedure {:yields} {:layer 5} {:refines "A_DoCopy"}
-  DoCopy({:linear "tid"} tid: Tid, creating_copy_bound: int);
-procedure {:right} {:layer 6}
+procedure {:right} {:layer 5}
   A_DoCopy({:linear "tid"} tid: Tid, creating_copy_bound: int)
 modifies copy_bound, copy;
 {
   assert is_running[copy_thread];
   assert tid == copy_thread;
   assert creating_copy_bound <= requested_copy_bound;
+  assert HoldsLockExclusive(tid, lock);
 
   if (creating_copy_bound == requested_copy_bound) {
     copy := latest;
@@ -196,36 +347,39 @@ modifies copy_bound, copy;
 // the return. Putting it in Copy_Stop seems a bit strange, but putting it outside
 // of Copy_Stop means that the lock is held even after setting is_running[tid] to false,
 // which also seems a bit strange.
-procedure {:yields} {:layer 6} {:refines "A_Copy"} Copy({:linear "tid"} tid: Tid)
-requires {:layer 6} requested_copy_bound > 0;
-requires {:layer 6} tid == copy_thread;
-requires {:layer 6} is_running[tid];
+procedure {:yields} {:layer 5} {:refines "A_Copy"} Copy({:linear "tid"} tid: Tid)
+requires {:layer 5} requested_copy_bound > 0;
+requires {:layer 5} tid == copy_thread;
+requires {:layer 5} is_running[tid];
 {
   var creating_copy_bound: int;
   creating_copy_bound := 0;
 
   yield;
-  assert {:layer 6} creating_copy_bound < requested_copy_bound;
-  assert {:layer 6} is_running[tid]; 
-  assert {:layer 6} tid == copy_thread;
+  assert {:layer 5} creating_copy_bound < requested_copy_bound;
+  assert {:layer 5} is_running[tid]; 
+  assert {:layer 5} tid == copy_thread;
+
+  call AcquireLockExclusive(tid);
 
   while (true)
-  invariant {:layer 6} {:terminates} true;
-  invariant {:layer 6} creating_copy_bound <= requested_copy_bound;
-  invariant {:layer 6} creating_copy_bound == requested_copy_bound ==>
+  invariant {:layer 5} {:terminates} true;
+  invariant {:layer 5} creating_copy_bound <= requested_copy_bound;
+  invariant {:layer 5} creating_copy_bound == requested_copy_bound ==>
     (copy == latest && copy_bound == requested_copy_bound);
+  invariant {:layer 4} HoldsLockExclusive(tid, lock); 
   {
     if (*) {
       call creating_copy_bound := Copy_Continue(creating_copy_bound);
     } else {
       call Copy_Stop(tid, creating_copy_bound);
+      call ReleaseLockExclusive(tid);
       yield;
       return;
     }
-
     call DoCopy(tid, creating_copy_bound);
   }
-  assert {:layer 6} false;
+  assert {:layer 5} false;
   yield;
 }
 
@@ -236,7 +390,7 @@ requires {:layer 6} is_running[tid];
 //
 // The above reasoning relies on the fact that there's at least one iteration of the
 // loop.
-procedure {:atomic} {:layer 7} A_Copy({:linear "tid"} tid: Tid)
+procedure {:atomic} {:layer 6, 10} A_Copy({:linear "tid"} tid: Tid)
 modifies copy, copy_bound, is_running;
 {
   copy := latest;
